Finish Ass 11

sf/Assignment11_10.v
@@ -4,23 +4,52 @@ Require Export Assignment11_09.
 
 (** Write a type checking function [tyeq: tm -> ty -> bool].
 **)
-
+Print tm.
 Fixpoint tycheck (t: tm) (T: ty) : bool :=
-  FILL_IN_HERE.
+  match t with
+  | ttrue => match T with
+             | TBool => true
+             | _ => false
+             end
+  | tfalse => match T with
+              | TBool => true
+              | _ => false
+              end
+  | tif t1 t2 t3 => if (andb (tycheck t1 TBool) (andb (tycheck t2 T) (tycheck t3 T))) then true else false
+  | tzero => match T with
+             | TNat => true
+             | _ => false
+             end
+  | tsucc t => if (tycheck t TNat) then match T with
+                                        | TNat => true
+                                        | _ => false
+                                        end
+                                   else false
+  | tpred t => if (tycheck t TNat) then match T with
+                                        | TNat => true
+                                        | _ => false
+                                        end
+                                   else false
+  | tiszero t => if (tycheck t TNat) then match T with
+                                          | TBool => true
+                                          | _ => false
+                                          end
+                                     else false
+end.
 
 Example tycheck_ex1:
   tycheck
     (tif (tiszero (tpred (tsucc (tsucc tzero)))) ttrue (tiszero (tsucc tzero))) 
     TBool 
   = true.
-Proof. exact FILL_IN_HERE. Qed.
+Proof. reflexivity. Qed.
 
 Example tycheck_ex2:
   tycheck
     (tif (tiszero (tpred (tsucc (tsucc tzero)))) tzero (tiszero (tsucc tzero))) 
     TBool 
   = false.
-Proof. exact FILL_IN_HERE. Qed.
+Proof. reflexivity. Qed.
 
 (** Prove that the type checking function [tyeq: tm -> ty -> bool] is correct.
 
@@ -33,14 +62,20 @@ Theorem tycheck_correct1: forall t T
     (TYCHK: tycheck t T = true),
   |- t \in T.
 Proof.
-  exact FILL_IN_HERE.
+  induction t; intros; destruct T; try constructor; try (solve by inversion);
+  inversion TYCHK; try (apply andb_prop in H0; destruct H0; clear H0;
+  apply andb_prop in H; destruct H; apply andb_prop in H0; destruct H0; auto);
+  destruct (tycheck t TNat) eqn:tc; try (solve by inversion); auto.  
 Qed.
 
 Theorem tycheck_correct2: forall t T
     (HASTY: |- t \in T),
   tycheck t T = true.
 Proof.
-  exact FILL_IN_HERE.
+  induction t; induction T; intros; auto; try solve by inversion;
+  try (inversion HASTY; subst; simpl; apply IHt1 in H2; apply IHt2 in H4; apply IHt3 in H5;
+  rewrite H2; rewrite H4; rewrite H5; reflexivity);
+  inversion HASTY; subst; apply IHt in H0; simpl; rewrite H0; reflexivity.
 Qed.
 
 (*-- Check --*)
