sf/Assignment11_03.v
@@ -9,7 +9,25 @@ Require Export Assignment11_02.
 Theorem step_deterministic:
   deterministic step.
 Proof with eauto.
-  exact FILL_IN_HERE.
+  unfold deterministic.
+  intros. generalize dependent y2. induction H; intros;
+  inversion H0; subst; try (solve by inversion); try reflexivity.
+  - rewrite (IHstep t1'0). reflexivity. assumption.
+  - rewrite (IHstep t1'0). reflexivity. assumption.
+  - assert (value t1). right. assumption.
+    apply value_is_nf in H1. unfold normal_form, not in H1.
+    inversion H2; subst. exfalso. apply H1...
+  - assert (value y2). right. assumption.
+    apply value_is_nf in H1. unfold normal_form, not in H1.
+    inversion H; subst. exfalso. apply H1...
+  - rewrite (IHstep t1'0). reflexivity. assumption.
+  - assert (value t1). right. assumption.
+    apply value_is_nf in H1. unfold normal_form, not in H1.
+    inversion H2; subst. exfalso. apply H1...
+  - assert (value t0). right. assumption.
+    apply value_is_nf in H1. unfold normal_form, not in H1.
+    inversion H; subst. exfalso. apply H1...
+  - rewrite (IHstep t1'0). reflexivity. assumption.
 Qed.
 
 (*-- Check --*)
