sf/Assignment11_05.v
@@ -28,11 +28,24 @@ Proof with auto.
     SCase "t1 can take a step".
       inversion H as [t1' H1].
       exists (tif t1' t2 t3)...
-      exact FILL_IN_HERE.
+  Case "T_Succ".
+    destruct IHHT.
+    apply (nat_canonical t1 HT) in H. inversion H; subst; clear H.
+    left...
+    left...
+    inversion H as [t1' H1]; right; eauto.
   Case "T_Pred".
-    exact FILL_IN_HERE.
+    destruct IHHT.
+    apply (nat_canonical t1 HT) in H. inversion H; subst; clear H.
+    right; eauto.
+    right; eauto.
+    inversion H as [t1' H1]; right; eauto.
   Case "T_Iszero".
-    exact FILL_IN_HERE.
+    destruct IHHT.
+    apply (nat_canonical t1 HT) in H. inversion H; subst; clear H.
+    right; eauto.
+    right; eauto.
+    inversion H as [t1' H1]; right; eauto.
 Qed.
 
 (*-- Check --*)
